towards tensorcore 2d with extraction

include/tensorcores.h
@@ -7,9 +7,13 @@ using namespace nvcuda;
 
 // Huge hack: krml generates an assignment that we don't really want,
 // so set it to 0.
-#define KPR_FRAGMENT_INIT(et, kind, m, n, k, layout)				\
-   (wmma::fragment<kind, m, n, k, et, layout>){0}
-#define KPR_FRAGMENT_INIT_C(et, kind, m, n, k)					\
-   (wmma::fragment<kind, m, n, k, et>){0}
+#define KPR_INIT(ty)\
+   (ty){0}
+#define KPR_FRAGMENT_TYPE(et, kind, m, n, k, layout) \
+   wmma::fragment<kind, m, n, k, et, layout>
+#define KPR_FRAGMENT_TYPE_C(et, kind, m, n, k) \
+   wmma::fragment<kind, m, n, k, et>
+#define KPR_ARRAY_FRAGMENT_TYPE(fragment_ty, size) \
+   fragment_ty[size]
 
 #endif /* __KUIPER_TENSORCORE_H */
